# 0001
Integral result rearrangement.

$$\tag{1}
\int \sin ax \ dx = - \frac{1}{a} \cos ax + c
$$

$$\tag{2}
\int_{x_1}^{x_2} \sin ax \ dx =  \left[ - \frac{1}{a} \cos ax \right]_{x = x_1}^{x_2}
$$

$$\tag{3}
\begin{array}{rcl}
\displaystyle \left[ - \frac{1}{a} \cos ax \right]_{x = x_1}^{x_2} & = & \displaystyle \left( - \frac{1}{a} \cos ax_2 \right) - \left( - \frac{1}{a} \cos ax_1 \right) \newline
& = & \displaystyle - \frac{1}{a} (\cos ax_2 - \cos ax_1) \newline
& = & \displaystyle - \frac{1}{a} [\cos ax]_{x = x_1}^{x_2}
\end{array}
$$


[&bull;](README.md)
[`0003`](../00/03.md)
