# 0014
Refresh about sigmoid function, the simplest form.

$$\tag{1}
\sigma(x) = \frac{1}{1 + e^{-x}}.
$$

Derivative of Eqn (1) is

$$\tag{2}
\sigma'(x) = \sigma(x) [ 1 - \sigma(x) ].
$$


Proof of Eqn (2) is as follow

$$\tag{3}
\begin{array}{rcl}
\displaystyle \frac{d\sigma}{dx} & = & \displaystyle \frac{d}{dx} \left( \frac{1}{1 + e^{-x}} \right) \newline
& = & \displaystyle \frac{d}{dx} \left( 1 + e^{-x} \right)^{-1} \newline
& = & \displaystyle -1 \cdot \left( 1 + e^{-x} \right)^{-2} \cdot \frac{d}{dx} \left( 1 + e^{-x} \right) \newline
& = & -1 \cdot \left( 1 + e^{-x} \right)^{-2} \cdot -1 \cdot e^{-x} \newline
& = & \left( 1 + e^{-x} \right)^{-2} e^{-x} \newline
& = & \displaystyle \left( \frac{1}{1 + e^{-x}} \right)^2 e^{-x} \newline
& = & \displaystyle \left( \frac{1}{1 + e^{-x}} \right) \left( \frac{e^{-x}}{1 + e^{-x}} \right) \newline
& = & \displaystyle \left( \frac{1}{1 + e^{-x}} \right) \left( \frac{1 + e^{-x} - 1}{1 + e^{-x}} \right) \newline
& = & \displaystyle \left( \frac{1}{1 + e^{-x}} \right) \left( \frac{1 + e^{-x}}{1 + e^{-x}} - \frac{1}{1 + e^{-x}} \right) \newline
& = & \displaystyle \left( \frac{1}{1 + e^{-x}} \right) \left( 1 - \frac{1}{1 + e^{-x}} \right) \newline
& = & s(x) [ 1 - s(x) ]
\end{array}
$$

Does it hold also for modified equation, e.g.

$$\tag{4}
\sigma(x) = \frac{A}{1 + e^{-k(x - x_0)}}?
$$


[&bull;](README.md)
[`0015`](../00/15.md)
