# 0031
Solve 3 uknowns with 3 equations for $N_1(x, y)$.

$$\tag{1}
\begin{array}{c}
a_1 + b_1 x_1 + c_1 y_1 = 1, \newline
a_1 + b_1 x_2 + c_1 y_2 = 0, \newline
a_1 + b_1 x_3 + c_1 y_3 = 0.
\end{array}
$$

$$\tag{2}
\begin{array}{rcl}
c_1 (y_2 - y_3) & = & b_1 (x_3 - x_2) \newline
c_1 & = & \displaystyle \left( \frac{x_3 - x_2}{y_2 - y_3} \right) \  b_1
\end{array}
$$

$$\tag{3}
\begin{array}{rcl}
c_1 (y_1 - y_2) & = & 1 + b_1 (x_2 - x_1) \newline
c_1 & = & \displaystyle \frac{1}{y_1 - y_2} + \left( \frac{x_2 - x_1}{y_1 - y_2} \right) \  b_1
\end{array}
$$

$$\tag{4}
\begin{array}{rcl}
\displaystyle \left( \frac{x_3 - x_2}{y_2 - y_3} \right) \  b_1 & = & \displaystyle \frac{1}{y_1 - y_2} + \left( \frac{x_2 - x_1}{y_1 - y_2} \right) \  b_1 \newline
\displaystyle \left( \frac{x_3 - x_2}{y_2 - y_3} - \frac{x_2 - x_1}{y_1 - y_2} \right) \  b_1 & = & \displaystyle \frac{1}{y_1 - y_2} \newline
\displaystyle \left[
\frac{ (x_3 - x_2)(y_1 - y_2) - (x_2 - x_1)(y_2 - y_3) }{ (y_2 - y_3)(y_1 - y_2) } \right] \  b_1 & = & \newline
b_1 & = & \displaystyle \left[ \frac{1}{y_1 - y_2} \frac{ (y_2 - y_3)(y_1 - y_2) }{ (x_3 - x_2)(y_1 - y_2) - (x_2 - x_1)(y_2 - y_3) } \right].
\end{array}
$$


---

$$\tag{2}
N_i(x_j, y_j) = \delta_{ij}.
$$

$$\tag{3}
N_i(x, y) = \frac{1}{2A}(a_i + b_i x + c_i y), \ \ i = 1, 2, 3.
$$

$$\tag{4}
\left[
\begin{array}{ccc}
1 & x_1 & y_1 \newline
1 & x_2 & y_2 \newline
1 & x_3 & y_3
\end{array}
\right]
\left[
\begin{array}{ccc}
a_1 & a_2 & a_3 \newline
b_1 & b_2 & b_3 \newline
c_1 & c_2 & c_3
\end{array}
\right]
=
2A
\left[
\begin{array}{ccc}
1 & 0 & 0 \newline
0 & 1 & 0 \newline
0 & 0 & 1
\end{array}
\right].
$$


[&bull;](README.md)
