# 0032
Solve 3 uknowns with 3 equations for $N_2(x, y)$ from $N_1(x, y)$.

$$\tag{1}
b_1 = \left[ \frac{ (y_2 - y_3) }{ (x_1 - x_2)(y_2 - y_3) - (x_2 - x_3)(y_1 - y_2) } \right].
$$

$$\tag{2}
c_1 = - b_1 \left( \frac{x_2 - x_3}{y_2 - y_3} \right).
$$

$$\tag{3}
a_1 = 1 - b_1 x_1 + c_1 y_1.
$$


$$\tag{4}
\begin{array}{c}
a_1 + b_1 x_1 + c_1 y_1 = 1, \newline
a_1 + b_1 x_2 + c_1 y_2 = 0, \newline
a_1 + b_1 x_3 + c_1 y_3 = 0.
\end{array}
$$

$$\tag{5}
\begin{array}{rcl}
c_1 (y_2 - y_3) & = & b_1 (x_3 - x_2) \newline
c_1 & = & \displaystyle \left( \frac{x_3 - x_2}{y_2 - y_3} \right) \  b_1
\end{array}
$$

$$\tag{6}
\begin{array}{rcl}
c_1 (y_1 - y_2) & = & 1 + b_1 (x_2 - x_1) \newline
c_1 & = & \displaystyle \frac{1}{y_1 - y_2} + \left( \frac{x_2 - x_1}{y_1 - y_2} \right) \  b_1
\end{array}
$$

$$
\begin{array}{rcl}
\displaystyle \left( \frac{x_3 - x_2}{y_2 - y_3} \right) \  b_1 & = & \displaystyle \frac{1}{y_1 - y_2} + \left( \frac{x_2 - x_1}{y_1 - y_2} \right) \  b_1 \newline
\displaystyle \left( \frac{x_3 - x_2}{y_2 - y_3} - \frac{x_2 - x_1}{y_1 - y_2} \right) \  b_1 & = & \displaystyle \frac{1}{y_1 - y_2} \newline
\end{array}
$$

$$\tag{7}
\begin{array}{c}
\displaystyle \left[
\frac{ (x_3 - x_2)(y_1 - y_2) - (x_2 - x_1)(y_2 - y_3) }{ (y_2 - y_3)(y_1 - y_2) } \right] \  b_1 = \frac{1}{y_1 - y_2} \newline
\displaystyle b_1 = \left[ \frac{ (y_2 - y_3) }{ (x_3 - x_2)(y_1 - y_2) - (x_2 - x_1)(y_2 - y_3) } \right].
\end{array}
$$


[&bull;](README.md)
